src/ReactorModel/Objects/Reactor/ReactorType/Updatable.lean
@@ -15,8 +15,9 @@ theorem RootEqualUpTo.mem_ids_iff {cmp} {rtr₁ : α} (e : RootEqualUpTo cmp i r
   exact ⟨(e h ▸ ·), (e h ▸ ·)⟩   
 
 -- Note: Without ID-uniqueness this can be satisfied by updating exactly one of the occurrences of
---       the target.
-inductive LawfulMemUpdate (cmp : Component.Valued) (i : ID) (f : cmp.type → cmp.type) : α → α → Prop
+--       the target. Since we have a choice of which target we update, this type isn't a `Prop`. 
+--       (We need to be able to eliminate into `Type` in `Member.fromLawfulUpdate`).
+inductive LawfulMemUpdate (cmp : Component.Valued) (i : ID) (f : cmp.type → cmp.type) : α → α → Type
   | final : 
     (RootEqualUpTo cmp i rtr₁ rtr₂) → (cmp? cmp rtr₁ i = some o) → (cmp? cmp rtr₂ i = f o) → 
     LawfulMemUpdate cmp i f rtr₁ rtr₂
@@ -24,26 +25,14 @@ inductive LawfulMemUpdate (cmp : Component.Valued) (i : ID) (f : cmp.type → cm
     (RootEqualUpTo .rtr j rtr₁ rtr₂) → (cmp? .rtr rtr₁ j = some n₁) → (cmp? .rtr rtr₂ j = some n₂) → 
     (LawfulMemUpdate cmp i f n₁ n₂) → LawfulMemUpdate cmp i f rtr₁ rtr₂
 
-inductive LawfulUpdate (cmp : Component.Valued) (i : ID) (f : cmp.type → cmp.type) : α → α → Prop
+-- Note: This isn't a `Prop` because of the explanation on `LawfulMemUpdate`.
+inductive LawfulUpdate (cmp : Component.Valued) (i : ID) (f : cmp.type → cmp.type) : α → α → Type
   | update : (LawfulMemUpdate cmp i f rtr₁ rtr₂) → LawfulUpdate cmp i f rtr₁ rtr₂
   | notMem : (IsEmpty $ Member cmp i rtr)        → LawfulUpdate cmp i f rtr rtr
 
 def LawfulUpdate.lift [LawfulCoe α β] {rtr₁ rtr₂ : α} {cmp i f} 
     (u : LawfulUpdate cmp i f (rtr₁ : β) (rtr₂ : β)) : LawfulUpdate cmp i f rtr₁ rtr₂ :=
   sorry -- might need coe ∘ update = update ∘ coe which is part of LawfulUpdatableCoe
-
--- TODO: Should these Member defs/theorems actually be about `Updatable`?
-def Member.fromLawfulUpdate {rtr₁ rtr₂ : α} {cmp i f} (u : LawfulUpdate cmp i f rtr₁ rtr₂) : 
-    (Member c j rtr₂) → Member c j rtr₁
-  | final h  => final sorry 
-  | nest h l => sorry 
-
-theorem Member.Equivalent.from_lawfulUpdate 
-    {rtr₁ rtr₂ : α} {cmp i f} (u : LawfulUpdate cmp i f rtr₁ rtr₂) (m : Member c j rtr₂) : 
-    Member.Equivalent m (Member.fromLawfulUpdate u m) := by
-  induction m
-  case final => constructor
-  case nest e => sorry
 
 end
 
@@ -63,38 +52,5 @@ class LawfulUpdatableCoe (α β) [a : Updatable α] [b : Updatable β] extends L
 
 instance [Updatable α] [LawfulUpdatable β] [c : LawfulUpdatableCoe α β] : LawfulUpdatable α where
   lawful rtr cmp i f := c.update_coe_comm ▸ LawfulUpdatable.lawful (rtr : β) cmp i f |>.lift 
-
-/-
-intro c j
-    constructor
-    intro l₁ l₂
-    open ReactorType in
-    by_cases Nonempty (Member cmp i rtr.core)
-    case neg =>
-      suffices h : Member c j (rtr.core.update cmp i f) = Member c j rtr.core from
-        (cast_inj h).mp $ rtr.uniqueIDs.allEq (cast h l₁) (cast h l₂)
-      simp [Core.update, h]
-    case pos =>
-      generalize hl : h.some = l
-      have h : Member c j (rtr.core.update _ i f) = Member c j (Core.update.go _ i f l) := by
-        simp [hl, Core.update, h]
-      apply (cast_inj h).mp
-      set l₁' := cast h l₁
-      set l₂' := cast h l₂
-      cases l
-      case final =>
-        simp [Core.update.go] at l₁' l₂'
-        sorry
-      case nest =>
-        sorry
--/
-
-/-
-structure LawfulUpdate [Indexable α] 
-    (rtr₁ rtr₂ : α) (cmp : Component.Valued) (i : ID) (f : cmp.type → cmp.type) : Prop where
-  equiv     : rtr₁ ≈ rtr₂  
-  unchanged : (c ≠ cmp ∨ j ≠ i) → rtr₁[c][j] = rtr₂[c][j]
-  changed   : f <$> rtr₁[cmp][i] = rtr₂[cmp][i]
--/
 
 end ReactorType
